tuning

Weidenbach_Book/IsaSAT_Clauses.thy
@@ -484,33 +484,19 @@ definition fm_add_new_packed where
     RETURN (N, i)
   }\<close>
 
-definition packed where
-  \<open>packed N \<longleftrightarrow> dom_m N = mset [1..<Suc (Max_mset (add_mset 0 (dom_m N)))]\<close>
-
-lemma packed_enpty[simp]: \<open>packed fmempty\<close>
-  by (auto simp: packed_def)
-
 lemma append_and_length_fm_add_new_packed:
   \<open>(uncurry2 (RETURN ooo append_and_length), uncurry2 fm_add_new_packed)
      \<in> [\<lambda>((b, C), N). packed N]\<^sub>f
        bool_rel \<times>\<^sub>f (\<langle>Id\<rangle>list_rel) \<times>\<^sub>f (\<langle>Id\<rangle>clauses_l_fmat) \<rightarrow> \<langle>\<langle>Id\<rangle>clauses_l_fmat \<times>\<^sub>f nat_rel\<rangle>nres_rel\<close>
-  apply (intro frefI nres_relI)
-  apply (auto simp: fm_add_new_at_position_def list_fmap_rel_def Let_def
+  by (intro frefI nres_relI)
+    (force simp:  fm_add_new_at_position_def list_fmap_rel_def Let_def
       max_def nth_append append_and_length_def fm_add_new_packed_def get_fresh_index_packed_def
-      RETURN_RES_refine_iff RES_RETURN_RES packed_def
+      RETURN_RES_refine_iff RES_RETURN_RES (* packed_def *) Max_n_upt Max_insert_Max_dom_into_packed
+      Max_dom_alt_def[symmetric] Max_dom_fmupd_irrel
       intro!: RETURN_SPEC_refine
-      dest: multi_member_split
-      split: if_splits)
-        apply force
-       apply (smt Suc_leI atLeastLessThan_iff finite_atLeastLessThan finite_set_mset_mset_set insert_iff
-      less_Suc_eq set_mset_add_mset_insert)
-  apply force
-  apply force
-  apply force
-  apply (case_tac \<open>set_mset (dom_m bc) = {}\<close>)
-   apply force
-  apply force
-  using not_less by blast
+      intro: packed_in_dom_mI
+     (*  dest: multi_member_split *)
+      (* split: if_splits *))
 
 lemma fm_add_new_packed_hnr[sepref_fr_rules]:
   \<open>(uncurry2 append_and_length_code, uncurry2 fm_add_new_packed)
@@ -600,24 +586,14 @@ lemma append_and_length_u32_fm_add_new_packed:
   \<open>(uncurry2 append_and_length_u32, uncurry2 fm_add_new_packed)
      \<in> [\<lambda>((b, C), N). Max (insert 0 (set_mset (dom_m N))) < uint32_max \<and> packed N]\<^sub>f
      bool_rel \<times>\<^sub>f (\<langle>Id\<rangle>list_rel) \<times>\<^sub>f (\<langle>Id\<rangle>clauses_l_fmat) \<rightarrow> \<langle>\<langle>Id\<rangle>clauses_l_fmat \<times>\<^sub>f nat_rel\<rangle>nres_rel\<close>
-  (* TODO Tune proof *)
-  apply (intro frefI nres_relI)
-  apply (auto simp: fm_add_new_at_position_def list_fmap_rel_def Let_def
-      max_def nth_append append_and_length_u32_def fm_add_new_packed_def get_fresh_index_packed_def
-      RETURN_RES_refine_iff RES_RETURN_RES packed_def
+  by (intro frefI nres_relI)
+    (force simp: list_fmap_rel_def Let_def
+       nth_append append_and_length_u32_def fm_add_new_packed_def get_fresh_index_packed_def
+      RETURN_RES_refine_iff RES_RETURN_RES Max_dom_alt_def[symmetric] Max_dom_fmupd_irrel
       intro!: RETURN_SPEC_refine ASSERT_refine_left
-      dest: multi_member_split
+      dest: multi_member_split Max_dom_le
+      intro: packed_in_dom_mI
       split: if_splits)
-         apply (metis Suc_leI insert_iff set_mset_add_mset_insert set_mset_empty)
-        apply (auto dest: dest: multi_member_split; fail)
-       apply (smt Suc_leI atLeastLessThan_iff finite_atLeastLessThan finite_set_mset_mset_set
-      insert_iff less_Suc_eq set_mset_add_mset_insert)
-      apply (auto dest: dest: multi_member_split; fail)
-     apply (auto dest: dest: multi_member_split; fail)
-    apply (auto dest: dest: multi_member_split; fail)
-   apply (case_tac \<open>set_mset (dom_m bc) = {}\<close>)
-    apply ((auto; fail)+)[2]
-  using leD by blast
 
 definition fm_add_new_packed_fast where
   [simp, symmetric, isasat_fast]: \<open>fm_add_new_packed_fast = fm_add_new_packed\<close>
